Move sizeOf into Serialise.

src/dafny/ssz/Merkleise.dfy
@@ -21,22 +21,6 @@ include "BoolSeDes.dfy"
     import opened SSZ
     import opened Helpers
 
-    /** SizeOf.
-     *
-     *  @param  s   A serialisable object of type uintN or bool.
-     *  @returns    The number of bytes used by a serialised form of this type.
-     */
-    function sizeOf(s: Serialisable): nat
-        requires wellTyped(s) && s.tipe in {Uint8_, Bool_}
-        ensures 1 <= sizeOf(s) <= 32 && sizeOf(s) == |serialise(s)|
-        {
-            match s
-                case Bool(_,_) => 1
-                case Uint8(_,_) => 1
-                
-        }
-
-
     /** chunkCount.
      *
      *  @param  s   A serialisable object.
